move out ensemble

Clean/Examples/FibonacciWithChannels.lean
@@ -11,8 +11,7 @@ Prove e2e soundness and completeness of the table ensemble.
 import Clean.Circuit
 import Clean.Circuit.Extensions
 import Clean.Gadgets.Addition8.Theorems
-import Clean.Air.FlatComponent
-import Clean.Air.Balance
+import Clean.Air.FlatEnsemble
 open ByteUtils (mod256 floorDiv256)
 open Gadgets.Addition8 (Theorems.soundness Theorems.completeness_bool Theorems.completeness_add)
 open Air.Flat
@@ -29,327 +28,6 @@ variable {PublicIO : TypeMap} [ProvableType PublicIO]
 
 -- tables need to be instantiated with a concrete circuit, not a family of circuits
 -- this is achieved for any FormalCircuit* by witnessing the inputs and plugging them in
-
-structure Ensemble (F : Type) [Field F] (PublicIO : TypeMap) [ProvableType PublicIO] where
-  tables : List (Component F)
-  channels : List (RawChannel F)
-  verifier : GeneralFormalCircuit F PublicIO unit := .empty F PublicIO
-  verifier_length_zero : ∀ pi, verifier.localLength pi = 0 := by
-    simp only [GeneralFormalCircuit.empty, circuit_norm]
-
-lemma Ensemble.size_verifier {ens : Ensemble F PublicIO} :
-    ens.verifier.size = size PublicIO := by
-  simp [GeneralFormalCircuit.size_eq, ens.verifier_length_zero]
-
-structure EnsembleWitness (ens : Ensemble F PublicIO) where
-  tables : List (Table F)
-  data : ProverData F
-  publicInput : PublicIO F
-  same_length : ens.tables.length = tables.length
-  same_circuits : ∀ i (hi : i < ens.tables.length), ens.tables[i] = tables[i].component
-  same_data : ∀ table ∈ tables, table.data = data
-
-/-- it's convenient to define a `Table` for the verifier, to treat them in a unified way -/
-def EnsembleWitness.verifierTable {ens : Ensemble F PublicIO} (witness : EnsembleWitness ens) : Table F where
-  component := ⟨ ens.verifier ⟩
-  width := size PublicIO
-  -- it's important that this has one row, which contains the input,
-  -- since we want to "run" the verifier once to produce interactions,
-  -- and so that constraints etc are actually enforced
-  table := [witness.publicInput |> toElements |>.toArray]
-  data := witness.data
-  uniform_width := by simp
-
-def Ensemble.verifierTable (ens : Ensemble F PublicIO) : Component F :=
-  ⟨ ens.verifier ⟩
-
-def Ensemble.allTables (ens : Ensemble F PublicIO) : List (Component F) :=
-  ens.verifierTable :: ens.tables
-
-namespace EnsembleWitness
-variable {ens : Ensemble F PublicIO}
-
-def allTables (witness : EnsembleWitness ens) : List (Table F) :=
-  witness.verifierTable :: witness.tables
-
-@[circuit_norm] lemma data_eq_of_mem_allTables (witness : EnsembleWitness ens) :
-  ∀ table ∈ witness.allTables, table.data = witness.data := by
-  simp [allTables, verifierTable]
-  exact witness.same_data
-
-abbrev allTablesWitness (witness : EnsembleWitness ens) : Tables F where
-  tables := witness.allTables
-  data := witness.data
-  same_data := by
-    simp [allTables, verifierTable]
-    apply witness.same_data
-
-@[circuit_norm] lemma allTablesWitness_tables (witness : EnsembleWitness ens) :
-  witness.allTablesWitness.tables = witness.allTables := rfl
-@[circuit_norm] lemma allTablesWitness_data (witness : EnsembleWitness ens) :
-  witness.allTablesWitness.data = witness.data := rfl
-
-instance : CoeOut (EnsembleWitness ens) (Tables F) where
-  coe witness := witness.allTablesWitness
-
-lemma mem_allTables_of_mem_tables (witness : EnsembleWitness ens) {table : Table F} :
-    table ∈ witness.tables → table ∈ witness.allTables := by
-  simp_all [allTables]
-
-lemma mem_allTables_verifierTable (witness : EnsembleWitness ens) :
-    witness.verifierTable ∈ witness.allTables := by
-  simp [allTables]
-
-lemma forall_mem_allTables_iff (witness : EnsembleWitness ens)
-  (motive : Table F → Prop) :
-    (∀ table ∈ witness.allTables, motive table) ↔
-    motive witness.verifierTable ∧ (∀ table ∈ witness.tables, motive table) := by
-  simp [allTables]
-
-@[circuit_norm] lemma verifierTable_component (witness : EnsembleWitness ens) :
-  witness.verifierTable.component = ens.verifierTable := rfl
-@[circuit_norm] lemma verifierTable_table (witness : EnsembleWitness ens) :
-  witness.verifierTable.table = [witness.publicInput |> toElements |>.toArray] := rfl
-
-@[circuit_norm]
-lemma tables_map_component (witness : EnsembleWitness ens) :
-    witness.tables.map (·.component) = ens.tables := by
-  apply List.ext_getElem
-  · simp [witness.same_length]
-  intro i hi hi'
-  simp [witness.same_circuits i hi']
-
-@[circuit_norm]
-lemma allTables_map_component (witness : EnsembleWitness ens) :
-    witness.allTables.map (·.component) = ens.allTables := by
-  simp only [circuit_norm, allTables, Ensemble.allTables]
-
-lemma mem_tables_component_of_mem_tables {witness : EnsembleWitness ens} {table : Table F} :
-    table ∈ witness.tables → table.component ∈ ens.tables := by
-  rw [← witness.tables_map_component]
-  grind
-
-lemma mem_allTables_component_of_mem_allTables {witness : EnsembleWitness ens} {table : Table F} :
-    table ∈ witness.allTables → table.component ∈ ens.allTables := by
-  rw [← witness.allTables_map_component]
-  grind
-
-def Constraints {ens : Ensemble F PublicIO} (witness : EnsembleWitness ens) : Prop :=
-  ∀ table ∈ witness.allTables, table.Constraints
-
-def Assumptions {ens : Ensemble F PublicIO} (witness : EnsembleWitness ens) : Prop :=
-  ∀ table ∈ witness.allTables, table.Assumptions
-
-def interactions {ens : Ensemble F PublicIO} (witness : EnsembleWitness ens) : List (Interaction F) :=
-  (witness.allTables).flatMap (fun table => table.interactions)
-
-noncomputable def interactionsWith {ens : Ensemble F PublicIO} (witness : EnsembleWitness ens)
-    (channel : RawChannel F) : List (Interaction F) :=
-  witness.allTables.flatMap (·.interactionsWith channel)
-
-@[circuit_norm] lemma allTablesWitness_constraints {ens : Ensemble F PublicIO} (witness : EnsembleWitness ens) :
-    witness.allTablesWitness.Constraints ↔ ∀ table ∈ witness.allTables, table.Constraints := by
-  simp only [Tables.Constraints]
-
-@[circuit_norm] lemma allTablesWitness_assumptions {ens : Ensemble F PublicIO} (witness : EnsembleWitness ens) :
-    witness.allTablesWitness.Assumptions ↔ ∀ table ∈ witness.allTables, table.Assumptions := by
-  simp only [Tables.Assumptions]
-
-@[circuit_norm] lemma interactionsWith_allTablesWitness {ens : Ensemble F PublicIO}
-  (witness : EnsembleWitness ens) (channel : RawChannel F) :
-    witness.allTablesWitness.interactionsWith channel = witness.interactionsWith channel := rfl
-end EnsembleWitness
-
-namespace Ensemble
-variable {ens : Ensemble F PublicIO}
-
-@[circuit_norm] lemma verifierTable_circuit : ens.verifierTable.circuit = ens.verifier := rfl
-@[circuit_norm] lemma verifierTable_input : ens.verifierTable.Input = PublicIO := rfl
-@[circuit_norm] lemma verifierTable_output : ens.verifierTable.Output = unit := rfl
-
-@[circuit_norm] lemma mem_allTables_verifierTable:
-  ens.verifierTable ∈ ens.allTables := by simp [allTables]
-
-lemma verifierTable_ext {ens1 ens2 : Ensemble F PublicIO} {witness1 : EnsembleWitness ens1} {witness2 : EnsembleWitness ens2} :
-    ens1.verifier = ens2.verifier →
-    witness1.publicInput = witness2.publicInput →
-    witness1.data = witness2.data →
-      witness1.verifierTable = witness2.verifierTable := by
-  rintro h_circuit h_input h_data
-  simp [EnsembleWitness.verifierTable, h_circuit, h_input, h_data]
-
-@[circuit_norm]
-abbrev verifierOperations (ens : Ensemble F PublicIO) : Operations F :=
-  (ens.verifier.main (varFromOffset PublicIO 0)).operations (size PublicIO)
-
-def VerifierConstraints (ens : Ensemble F PublicIO) (publicInput : PublicIO F) (data : ProverData F) : Prop :=
-  ens.verifierOperations.ConstraintsHold (.fromInput publicInput data)
-
-def VerifierGuarantees (ens : Ensemble F PublicIO) (publicInput : PublicIO F) (data : ProverData F) : Prop :=
-  ens.verifierOperations.FullGuarantees (.fromInput publicInput data)
-
-@[circuit_norm]
-def VerifierSpec (ens : Ensemble F PublicIO) (publicInput : PublicIO F) (data : ProverData F) : Prop :=
-  ens.verifier.Spec publicInput () data
-
-lemma verifierTable_constraints :
-  ens.verifierTable.operations.constraints = ens.verifierOperations.constraints := by
-  rw [Component.constraints_eq]
-  simp only [circuit_norm]
-
-lemma verifierTable_lookups :
-  ens.verifierTable.operations.lookups = ens.verifierOperations.lookups := by
-  rw [Component.lookups_eq]
-  simp only [circuit_norm]
-
-lemma verifierTable_interactions :
-  ens.verifierTable.operations.interactions = ens.verifierOperations.interactions := by
-  rw [Component.interactions_eq]
-  simp only [circuit_norm]
-
-lemma verifierTable_interactionsWith {channel : RawChannel F} :
-  ens.verifierTable.operations.interactionsWith channel =
-    ens.verifierOperations.interactionsWith channel := by
-  rw [Component.interactionsWith_eq]
-  simp only [circuit_norm]
-end Ensemble
-
-namespace EnsembleWitness
-variable {ens : Ensemble F PublicIO}
-
-lemma mem_interactionsWith {witness : EnsembleWitness ens}
-  {channel : RawChannel F} {i : Interaction F} :
-    i ∈ witness.interactionsWith channel ↔
-    ∃ table ∈ witness.allTables, i ∈ table.interactionsWith channel := by
-  simp only [interactionsWith, List.mem_flatMap]
-
-lemma channel_eq_of_mem_interactionsWith {witness : EnsembleWitness ens}
-  {channel : RawChannel F} {i : Interaction F} :
-    i ∈ witness.interactionsWith channel → i.channel = channel := by
-  rw [mem_interactionsWith]
-  intro h_mem
-  rcases h_mem with ⟨ table, h_table, h_mem_table ⟩
-  apply table.channel_eq_of_mem_interactionsWith h_mem_table
-
-@[circuit_norm]
-lemma verifierTable_forall {witness : EnsembleWitness ens}
-      {motive : Array F → Prop} :
-    (∀ row ∈ witness.verifierTable.table, motive row) ↔ motive (toElements witness.publicInput).toArray := by
-  simp [verifierTable]
-
-@[circuit_norm]
-lemma verifierTable_flatMap {witness : EnsembleWitness ens}
-      {α : Type*} {f : Array F → List α} :
-    witness.verifierTable.table.flatMap f = f (toElements witness.publicInput).toArray := by
-  simp [verifierTable]
-
-@[circuit_norm]
-lemma verifierTable_environment {witness : EnsembleWitness ens} {publicInput : PublicIO F} :
-    witness.verifierTable.environment (toElements publicInput).toArray =
-      Environment.fromInput publicInput witness.data := rfl
-
-lemma verifierConstraints_iff_verifierTable_constraints {witness : EnsembleWitness ens} :
-  ens.VerifierConstraints witness.publicInput witness.data ↔
-    witness.verifierTable.Constraints := by
-  simp only [Ensemble.VerifierConstraints, Table.Constraints]
-  simp only [circuit_norm, Ensemble.verifierTable_constraints, Ensemble.verifierTable_lookups]
-
-lemma verifierAssumptions_iff_verifierTable_assumptions {witness : EnsembleWitness ens} :
-  ens.verifier.Assumptions witness.publicInput witness.data ↔
-    witness.verifierTable.Assumptions := by
-  simp only [circuit_norm, Table.Assumptions,
-    Ensemble.verifierTable, Component.Assumptions]
-
-lemma verifierGuarantees_iff_verifierTable_guarantees {witness : EnsembleWitness ens} :
-  ens.VerifierGuarantees witness.publicInput witness.data ↔
-    witness.verifierTable.Guarantees := by
-  simp only [Ensemble.VerifierGuarantees, Table.Guarantees]
-  simp only [circuit_norm, Ensemble.verifierTable_interactions]
-
-lemma verifierChannelRequirements_iff {witness : EnsembleWitness ens} {channel : RawChannel F} :
-  ens.verifierOperations.ChannelRequirements channel (.fromInput witness.publicInput witness.data) ↔
-    witness.verifierTable.ChannelRequirements channel := by
-  simp only [Table.ChannelRequirements, circuit_norm, Ensemble.verifierTable_interactions]
-
-lemma verifierConstraints_of_constraints {ens : Ensemble F PublicIO} {witness : EnsembleWitness ens} :
-  witness.Constraints →
-    ens.VerifierConstraints witness.publicInput witness.data := by
-  rw [verifierConstraints_iff_verifierTable_constraints, Constraints, EnsembleWitness.forall_mem_allTables_iff]
-  simp_all
-
-lemma verifierAssumptions_of_assumptions {ens : Ensemble F PublicIO} {witness : EnsembleWitness ens} :
-  witness.Assumptions →
-    ens.verifier.Assumptions witness.publicInput witness.data := by
-  rw [verifierAssumptions_iff_verifierTable_assumptions, Assumptions, forall_mem_allTables_iff]
-  simp_all
-
-lemma interactionsWith_of_verifier_empty {ens : Ensemble F PublicIO} {witness : EnsembleWitness ens} {channel : RawChannel F}
-  (h_verifier_empty : ens.verifier = .empty F PublicIO) :
-    witness.interactionsWith channel = witness.tables.flatMap (·.interactionsWith channel) := by
-  simp [interactionsWith, allTables, Table.interactionsWith,
-    Ensemble.verifierTable_interactionsWith, circuit_norm, h_verifier_empty]
-
-lemma verifierTable_constraints_of_verifier_empty {ens : Ensemble F PublicIO} {witness : EnsembleWitness ens}
-  (h_verifier_empty : ens.verifier = .empty F PublicIO) :
-    witness.verifierTable.Constraints := by
-  rw [← verifierConstraints_iff_verifierTable_constraints]
-  simp only [Ensemble.VerifierConstraints, circuit_norm, h_verifier_empty]
-
-lemma verifierTable_assumptions_of_verifier_empty {ens : Ensemble F PublicIO} {witness : EnsembleWitness ens}
-  (h_verifier_empty : ens.verifier = .empty F PublicIO) :
-    witness.verifierTable.Assumptions := by
-  rw [← verifierAssumptions_iff_verifierTable_assumptions]
-  simp only [circuit_norm, h_verifier_empty]
-
-/-- The ensemble interactions with a particular channel are balanced. -/
-@[circuit_norm]
-abbrev BalancedChannel [DecidableEq F] {ens : Ensemble F PublicIO} (witness : EnsembleWitness ens)
-    (channel : RawChannel F) : Prop :=
-  BalancedInteractions (witness.allTablesWitness.interactionsWith channel)
-
-/-- All ensemble interactions with all ensemble channels are balanced. -/
-@[circuit_norm]
-def BalancedChannels [DecidableEq F] {ens : Ensemble F PublicIO} (witness : EnsembleWitness ens) : Prop :=
-  ∀ channel ∈ ens.channels, BalancedChannel witness channel
-end EnsembleWitness
-
-namespace Ensemble
-variable [DecidableEq F]
-
-/--
-The raw "statement" that a proof about an ensemble makes. Could also be called "relation".
-
-TODO: we currently assume a proof system that already provides us with the fact that the
-total interaction length doesn't overflow (as part of `BalancedChannels`).
-
-In practice, however, it's not the total interaction length that is part of a proof,
-but rather the length of each individual table. It should be our verifier's job to
-verify a bound on the interaction length from the given table lengths.
--/
-def Statement (ens : Ensemble F PublicIO) (publicInput : PublicIO F) : Prop :=
-  ∃ witness : EnsembleWitness ens,
-    witness.publicInput = publicInput ∧
-    witness.Constraints ∧
-    witness.BalancedChannels
-
-/-- Soundness: assumptions plus the raw statement imply the spec. -/
-def Soundness (ens : Ensemble F PublicIO) (Assumptions Spec : PublicIO F → Prop) : Prop :=
-  ∀ publicInput, Assumptions publicInput → ens.Statement publicInput → Spec publicInput
-
-/--
-Completeness: assumptions plus the spec implies the raw statement.
--/
-def Completeness (ens : Ensemble F PublicIO) (Assumptions Spec : PublicIO F → Prop) : Prop :=
-  ∀ publicInput, Assumptions publicInput → Spec publicInput → ens.Statement publicInput
-end Ensemble
-
-structure FormalEnsemble (F : Type) [Field F] [DecidableEq F]
-    (PublicIO : TypeMap) [ProvableType PublicIO] where
-  ensemble : Ensemble F PublicIO
-  Assumptions : PublicIO F → Prop := fun _ => True
-  Spec : PublicIO F → Prop
-  soundness : ensemble.Soundness Assumptions Spec
-  -- completeness : ensemble.Completeness Assumptions Spec
 
 -- infrastructure for iteratively adding tables to an ensemble such that we can always fill in
 -- the next table's guarantees
@@ -874,6 +552,7 @@ lemma soundChannels_cons_of_soundChannels [DecidableEq F] {tables : List (Compon
   · simp
   simp_all [SoundChannels]
 
+namespace Air.Flat
 namespace EnsembleWitness
 @[circuit_norm]
 abbrev PartialBalancedChannels [DecidableEq F] {ens : Ensemble F PublicIO} (finished : List (RawChannel F))
@@ -1433,6 +1112,7 @@ lemma Component.interactionsWith_of_exposedChannels {table : Component F} {chann
   rw [Component.interactionsWith_eq]
   simp only [circuit_norm, Component.exposedChannels] at *
   convert table.circuit.interactionsWith_eq_of_mem_exposedChannels _ _ _ h_exposed
+end Air.Flat
 
 def List.flattenPairs {α : Type} (pairs : List (α × α)) : List α :=
   pairs.map (fun (a, b) => [a, b]) |>.flatten
@@ -1468,14 +1148,14 @@ lemma flatMap_flatMap {α β γ : Type*} (l : List γ) (g : γ → List α) (f :
     simp [ih]
     rfl
 
-namespace Air.Flat.Table
+namespace Air.Flat
 
+namespace Table
 noncomputable def interactionssWith (table : Table F)
     (channel : RawChannel F) : List (List (Interaction F)) :=
   table.table.map fun row =>
     table.component.operations.interactionValuesWith channel (table.environment row)
-
-end Air.Flat.Table
+end Table
 
 /-- Ensemble interactions preserving the per-row structure until the final flatten. -/
 lemma EnsembleWitness.flatMap_interactionsWith_eq_flatten {ens : Ensemble F PublicIO}
@@ -2019,6 +1699,7 @@ variable {soundEns : SoundEnsemble F PublicIO} {vm : VmTables F PublicIO}
   (soundEns.addVm vm nmv gsf rdf).ensemble = soundEns.ensemble.addVm vm := rfl
 
 end SoundEnsemble
+end Air.Flat
 end
 
 -- CONCRETE EXAMPLE STARTS HERE
