Clean/Air/FlatEnsemble.lean
@@ -1,0 +1,333 @@
+/-
+This file defines flat AIR ensembles and what soundness and completeness mean for them.
+-/
+import Clean.Air.FlatComponent
+import Clean.Air.Balance
+
+namespace Air.Flat
+variable {F : Type} [Field F]
+variable {PublicIO : TypeMap} [ProvableType PublicIO]
+
+structure Ensemble (F : Type) [Field F] (PublicIO : TypeMap) [ProvableType PublicIO] where
+  tables : List (Component F)
+  channels : List (RawChannel F)
+  -- TODO: the verifier shouldn't be treated as a "circuit", and possibly shouldn't even be on here
+  verifier : GeneralFormalCircuit F PublicIO unit := .empty F PublicIO
+  verifier_length_zero : ∀ pi, verifier.localLength pi = 0 := by
+    simp only [GeneralFormalCircuit.empty, circuit_norm]
+
+lemma Ensemble.size_verifier {ens : Ensemble F PublicIO} :
+    ens.verifier.size = size PublicIO := by
+  simp [GeneralFormalCircuit.size_eq, ens.verifier_length_zero]
+
+structure EnsembleWitness (ens : Ensemble F PublicIO) where
+  tables : List (Table F)
+  data : ProverData F
+  publicInput : PublicIO F
+  same_length : ens.tables.length = tables.length
+  same_circuits : ∀ i (hi : i < ens.tables.length), ens.tables[i] = tables[i].component
+  same_data : ∀ table ∈ tables, table.data = data
+
+/-- it's convenient to define a `Table` for the verifier, to treat them in a unified way -/
+def EnsembleWitness.verifierTable {ens : Ensemble F PublicIO} (witness : EnsembleWitness ens) : Table F where
+  component := ⟨ ens.verifier ⟩
+  width := size PublicIO
+  -- it's important that this has one row, which contains the input,
+  -- since we want to "run" the verifier once to produce interactions,
+  -- and so that constraints etc are actually enforced
+  table := [witness.publicInput |> toElements |>.toArray]
+  data := witness.data
+  uniform_width := by simp
+
+def Ensemble.verifierTable (ens : Ensemble F PublicIO) : Component F :=
+  ⟨ ens.verifier ⟩
+
+def Ensemble.allTables (ens : Ensemble F PublicIO) : List (Component F) :=
+  ens.verifierTable :: ens.tables
+
+namespace EnsembleWitness
+variable {ens : Ensemble F PublicIO}
+
+def allTables (witness : EnsembleWitness ens) : List (Table F) :=
+  witness.verifierTable :: witness.tables
+
+@[circuit_norm] lemma data_eq_of_mem_allTables (witness : EnsembleWitness ens) :
+  ∀ table ∈ witness.allTables, table.data = witness.data := by
+  simp [allTables, verifierTable]
+  exact witness.same_data
+
+abbrev allTablesWitness (witness : EnsembleWitness ens) : Tables F where
+  tables := witness.allTables
+  data := witness.data
+  same_data := by
+    simp [allTables, verifierTable]
+    apply witness.same_data
+
+@[circuit_norm] lemma allTablesWitness_tables (witness : EnsembleWitness ens) :
+  witness.allTablesWitness.tables = witness.allTables := rfl
+@[circuit_norm] lemma allTablesWitness_data (witness : EnsembleWitness ens) :
+  witness.allTablesWitness.data = witness.data := rfl
+
+instance : CoeOut (EnsembleWitness ens) (Tables F) where
+  coe witness := witness.allTablesWitness
+
+lemma mem_allTables_of_mem_tables (witness : EnsembleWitness ens) {table : Table F} :
+    table ∈ witness.tables → table ∈ witness.allTables := by
+  simp_all [allTables]
+
+lemma mem_allTables_verifierTable (witness : EnsembleWitness ens) :
+    witness.verifierTable ∈ witness.allTables := by
+  simp [allTables]
+
+lemma forall_mem_allTables_iff (witness : EnsembleWitness ens)
+  (motive : Table F → Prop) :
+    (∀ table ∈ witness.allTables, motive table) ↔
+    motive witness.verifierTable ∧ (∀ table ∈ witness.tables, motive table) := by
+  simp [allTables]
+
+@[circuit_norm] lemma verifierTable_component (witness : EnsembleWitness ens) :
+  witness.verifierTable.component = ens.verifierTable := rfl
+@[circuit_norm] lemma verifierTable_table (witness : EnsembleWitness ens) :
+  witness.verifierTable.table = [witness.publicInput |> toElements |>.toArray] := rfl
+
+@[circuit_norm]
+lemma tables_map_component (witness : EnsembleWitness ens) :
+    witness.tables.map (·.component) = ens.tables := by
+  apply List.ext_getElem
+  · simp [witness.same_length]
+  intro i hi hi'
+  simp [witness.same_circuits i hi']
+
+@[circuit_norm]
+lemma allTables_map_component (witness : EnsembleWitness ens) :
+    witness.allTables.map (·.component) = ens.allTables := by
+  simp only [circuit_norm, allTables, Ensemble.allTables]
+
+lemma mem_tables_component_of_mem_tables {witness : EnsembleWitness ens} {table : Table F} :
+    table ∈ witness.tables → table.component ∈ ens.tables := by
+  rw [← witness.tables_map_component]
+  grind
+
+lemma mem_allTables_component_of_mem_allTables {witness : EnsembleWitness ens} {table : Table F} :
+    table ∈ witness.allTables → table.component ∈ ens.allTables := by
+  rw [← witness.allTables_map_component]
+  grind
+
+def Constraints {ens : Ensemble F PublicIO} (witness : EnsembleWitness ens) : Prop :=
+  ∀ table ∈ witness.allTables, table.Constraints
+
+def Assumptions {ens : Ensemble F PublicIO} (witness : EnsembleWitness ens) : Prop :=
+  ∀ table ∈ witness.allTables, table.Assumptions
+
+def interactions {ens : Ensemble F PublicIO} (witness : EnsembleWitness ens) : List (Interaction F) :=
+  (witness.allTables).flatMap (fun table => table.interactions)
+
+noncomputable def interactionsWith {ens : Ensemble F PublicIO} (witness : EnsembleWitness ens)
+    (channel : RawChannel F) : List (Interaction F) :=
+  witness.allTables.flatMap (·.interactionsWith channel)
+
+@[circuit_norm] lemma allTablesWitness_constraints {ens : Ensemble F PublicIO} (witness : EnsembleWitness ens) :
+    witness.allTablesWitness.Constraints ↔ ∀ table ∈ witness.allTables, table.Constraints := by
+  simp only [Tables.Constraints]
+
+@[circuit_norm] lemma allTablesWitness_assumptions {ens : Ensemble F PublicIO} (witness : EnsembleWitness ens) :
+    witness.allTablesWitness.Assumptions ↔ ∀ table ∈ witness.allTables, table.Assumptions := by
+  simp only [Tables.Assumptions]
+
+@[circuit_norm] lemma interactionsWith_allTablesWitness {ens : Ensemble F PublicIO}
+  (witness : EnsembleWitness ens) (channel : RawChannel F) :
+    witness.allTablesWitness.interactionsWith channel = witness.interactionsWith channel := rfl
+end EnsembleWitness
+
+namespace Ensemble
+variable {ens : Ensemble F PublicIO}
+
+@[circuit_norm] lemma verifierTable_circuit : ens.verifierTable.circuit = ens.verifier := rfl
+@[circuit_norm] lemma verifierTable_input : ens.verifierTable.Input = PublicIO := rfl
+@[circuit_norm] lemma verifierTable_output : ens.verifierTable.Output = unit := rfl
+
+@[circuit_norm] lemma mem_allTables_verifierTable:
+  ens.verifierTable ∈ ens.allTables := by simp [allTables]
+
+lemma verifierTable_ext {ens1 ens2 : Ensemble F PublicIO} {witness1 : EnsembleWitness ens1} {witness2 : EnsembleWitness ens2} :
+    ens1.verifier = ens2.verifier →
+    witness1.publicInput = witness2.publicInput →
+    witness1.data = witness2.data →
+      witness1.verifierTable = witness2.verifierTable := by
+  rintro h_circuit h_input h_data
+  simp [EnsembleWitness.verifierTable, h_circuit, h_input, h_data]
+
+@[circuit_norm]
+abbrev verifierOperations (ens : Ensemble F PublicIO) : Operations F :=
+  (ens.verifier.main (varFromOffset PublicIO 0)).operations (size PublicIO)
+
+def VerifierConstraints (ens : Ensemble F PublicIO) (publicInput : PublicIO F) (data : ProverData F) : Prop :=
+  ens.verifierOperations.ConstraintsHold (.fromInput publicInput data)
+
+def VerifierGuarantees (ens : Ensemble F PublicIO) (publicInput : PublicIO F) (data : ProverData F) : Prop :=
+  ens.verifierOperations.FullGuarantees (.fromInput publicInput data)
+
+@[circuit_norm]
+def VerifierSpec (ens : Ensemble F PublicIO) (publicInput : PublicIO F) (data : ProverData F) : Prop :=
+  ens.verifier.Spec publicInput () data
+
+lemma verifierTable_constraints :
+  ens.verifierTable.operations.constraints = ens.verifierOperations.constraints := by
+  rw [Component.constraints_eq]
+  simp only [circuit_norm]
+
+lemma verifierTable_lookups :
+  ens.verifierTable.operations.lookups = ens.verifierOperations.lookups := by
+  rw [Component.lookups_eq]
+  simp only [circuit_norm]
+
+lemma verifierTable_interactions :
+  ens.verifierTable.operations.interactions = ens.verifierOperations.interactions := by
+  rw [Component.interactions_eq]
+  simp only [circuit_norm]
+
+lemma verifierTable_interactionsWith {channel : RawChannel F} :
+  ens.verifierTable.operations.interactionsWith channel =
+    ens.verifierOperations.interactionsWith channel := by
+  rw [Component.interactionsWith_eq]
+  simp only [circuit_norm]
+end Ensemble
+
+namespace EnsembleWitness
+variable {ens : Ensemble F PublicIO}
+
+lemma mem_interactionsWith {witness : EnsembleWitness ens}
+  {channel : RawChannel F} {i : Interaction F} :
+    i ∈ witness.interactionsWith channel ↔
+    ∃ table ∈ witness.allTables, i ∈ table.interactionsWith channel := by
+  simp only [interactionsWith, List.mem_flatMap]
+
+lemma channel_eq_of_mem_interactionsWith {witness : EnsembleWitness ens}
+  {channel : RawChannel F} {i : Interaction F} :
+    i ∈ witness.interactionsWith channel → i.channel = channel := by
+  rw [mem_interactionsWith]
+  intro h_mem
+  rcases h_mem with ⟨ table, h_table, h_mem_table ⟩
+  apply table.channel_eq_of_mem_interactionsWith h_mem_table
+
+@[circuit_norm]
+lemma verifierTable_forall {witness : EnsembleWitness ens}
+      {motive : Array F → Prop} :
+    (∀ row ∈ witness.verifierTable.table, motive row) ↔ motive (toElements witness.publicInput).toArray := by
+  simp [verifierTable]
+
+@[circuit_norm]
+lemma verifierTable_flatMap {witness : EnsembleWitness ens}
+      {α : Type*} {f : Array F → List α} :
+    witness.verifierTable.table.flatMap f = f (toElements witness.publicInput).toArray := by
+  simp [verifierTable]
+
+@[circuit_norm]
+lemma verifierTable_environment {witness : EnsembleWitness ens} {publicInput : PublicIO F} :
+    witness.verifierTable.environment (toElements publicInput).toArray =
+      Environment.fromInput publicInput witness.data := rfl
+
+lemma verifierConstraints_iff_verifierTable_constraints {witness : EnsembleWitness ens} :
+  ens.VerifierConstraints witness.publicInput witness.data ↔
+    witness.verifierTable.Constraints := by
+  simp only [Ensemble.VerifierConstraints, Table.Constraints]
+  simp only [circuit_norm, Ensemble.verifierTable_constraints, Ensemble.verifierTable_lookups]
+
+lemma verifierAssumptions_iff_verifierTable_assumptions {witness : EnsembleWitness ens} :
+  ens.verifier.Assumptions witness.publicInput witness.data ↔
+    witness.verifierTable.Assumptions := by
+  simp only [circuit_norm, Table.Assumptions,
+    Ensemble.verifierTable, Component.Assumptions]
+
+lemma verifierGuarantees_iff_verifierTable_guarantees {witness : EnsembleWitness ens} :
+  ens.VerifierGuarantees witness.publicInput witness.data ↔
+    witness.verifierTable.Guarantees := by
+  simp only [Ensemble.VerifierGuarantees, Table.Guarantees]
+  simp only [circuit_norm, Ensemble.verifierTable_interactions]
+
+lemma verifierChannelRequirements_iff {witness : EnsembleWitness ens} {channel : RawChannel F} :
+  ens.verifierOperations.ChannelRequirements channel (.fromInput witness.publicInput witness.data) ↔
+    witness.verifierTable.ChannelRequirements channel := by
+  simp only [Table.ChannelRequirements, circuit_norm, Ensemble.verifierTable_interactions]
+
+lemma verifierConstraints_of_constraints {ens : Ensemble F PublicIO} {witness : EnsembleWitness ens} :
+  witness.Constraints →
+    ens.VerifierConstraints witness.publicInput witness.data := by
+  rw [verifierConstraints_iff_verifierTable_constraints, Constraints, EnsembleWitness.forall_mem_allTables_iff]
+  simp_all
+
+lemma verifierAssumptions_of_assumptions {ens : Ensemble F PublicIO} {witness : EnsembleWitness ens} :
+  witness.Assumptions →
+    ens.verifier.Assumptions witness.publicInput witness.data := by
+  rw [verifierAssumptions_iff_verifierTable_assumptions, Assumptions, forall_mem_allTables_iff]
+  simp_all
+
+lemma interactionsWith_of_verifier_empty {ens : Ensemble F PublicIO} {witness : EnsembleWitness ens} {channel : RawChannel F}
+  (h_verifier_empty : ens.verifier = .empty F PublicIO) :
+    witness.interactionsWith channel = witness.tables.flatMap (·.interactionsWith channel) := by
+  simp [interactionsWith, allTables, Table.interactionsWith,
+    Ensemble.verifierTable_interactionsWith, circuit_norm, h_verifier_empty]
+
+lemma verifierTable_constraints_of_verifier_empty {ens : Ensemble F PublicIO} {witness : EnsembleWitness ens}
+  (h_verifier_empty : ens.verifier = .empty F PublicIO) :
+    witness.verifierTable.Constraints := by
+  rw [← verifierConstraints_iff_verifierTable_constraints]
+  simp only [Ensemble.VerifierConstraints, circuit_norm, h_verifier_empty]
+
+lemma verifierTable_assumptions_of_verifier_empty {ens : Ensemble F PublicIO} {witness : EnsembleWitness ens}
+  (h_verifier_empty : ens.verifier = .empty F PublicIO) :
+    witness.verifierTable.Assumptions := by
+  rw [← verifierAssumptions_iff_verifierTable_assumptions]
+  simp only [circuit_norm, h_verifier_empty]
+
+/-- The ensemble interactions with a particular channel are balanced. -/
+@[circuit_norm]
+abbrev BalancedChannel [DecidableEq F] {ens : Ensemble F PublicIO} (witness : EnsembleWitness ens)
+    (channel : RawChannel F) : Prop :=
+  BalancedInteractions (witness.allTablesWitness.interactionsWith channel)
+
+/-- All ensemble interactions with all ensemble channels are balanced. -/
+@[circuit_norm]
+def BalancedChannels [DecidableEq F] {ens : Ensemble F PublicIO} (witness : EnsembleWitness ens) : Prop :=
+  ∀ channel ∈ ens.channels, BalancedChannel witness channel
+end EnsembleWitness
+
+namespace Ensemble
+variable [DecidableEq F]
+
+/--
+The raw "statement" that a proof about an ensemble makes. Could also be called "relation".
+
+TODO: we currently assume a proof system that already provides us with the fact that the
+total interaction length doesn't overflow (as part of `BalancedChannels`).
+
+In practice, however, it's not the total interaction length that is part of a proof,
+but rather the length of each individual table. It should be our verifier's job to
+verify a bound on the interaction length from the given table lengths.
+-/
+def Statement (ens : Ensemble F PublicIO) (publicInput : PublicIO F) : Prop :=
+  ∃ witness : EnsembleWitness ens,
+    witness.publicInput = publicInput ∧
+    witness.Constraints ∧
+    witness.BalancedChannels
+
+/-- Soundness: assumptions plus the raw statement imply the spec. -/
+def Soundness (ens : Ensemble F PublicIO) (Assumptions Spec : PublicIO F → Prop) : Prop :=
+  ∀ publicInput, Assumptions publicInput → ens.Statement publicInput → Spec publicInput
+
+/--
+Completeness: assumptions plus the spec implies the raw statement.
+-/
+def Completeness (ens : Ensemble F PublicIO) (Assumptions Spec : PublicIO F → Prop) : Prop :=
+  ∀ publicInput, Assumptions publicInput → Spec publicInput → ens.Statement publicInput
+end Ensemble
+
+structure FormalEnsemble (F : Type) [Field F] [DecidableEq F]
+    (PublicIO : TypeMap) [ProvableType PublicIO] where
+  ensemble : Ensemble F PublicIO
+  Assumptions : PublicIO F → Prop := fun _ => True
+  Spec : PublicIO F → Prop
+  soundness : ensemble.Soundness Assumptions Spec
+  -- completeness : ensemble.Completeness Assumptions Spec
+
+end Air.Flat
